partial_abort/formalization/f_stepWF.v
@@ -1,0 +1,246 @@
+Require Export semantics.   
+
+Theorem validateHeapExtensionC : forall S L H S' H' new C, 
+                  Forall (fun x : location * term * stamp => getStamp x = C) new ->
+                  S < C ->
+                  validate S L H S' H' L commit ->
+                  (exists Hnew, validate S L (new++H) S' (Hnew++new++H) L commit) \/
+                  (exists Lnew e, validate S L (new++H) S' (new++H) Lnew (abort e) /\
+                             postfix Lnew L).
+Proof.
+  intros. remember commit. induction H2; try solve[inv Heqv]; clear Heqv. 
+  {left. exists nil. constructor. }
+  {copy H1. apply IHvalidate in H1; auto. inv H1.
+   {invertHyp. eapply LookupExtensionGE in H2. Focus 2. eauto. inv H2. 
+    {left. exists x. eapply validateCommitRead; eauto. }
+    {invertHyp. right. exists L0. exists (fill E (get (loc l))). split.
+     eapply validateAbortRead; eauto. omega. unfold postfix. exists [readItem l E]. auto. }
+   }
+   {invertHyp. right. exists x. exists x0. split. eapply validateAbortPropogate. eauto. 
+    unfold postfix in *. invertHyp. exists (readItem l E :: x1). auto. }
+  }
+  {copy H1. apply IHvalidate in H1; auto. inv H1. 
+   {invertHyp. left. exists ((l, v, S')::x). simpl. eapply validateWrite. auto. }
+   {invertHyp. right. exists x. exists x0. split. eapply validateAbortPropogate. auto. 
+    unfold postfix in *. invertHyp. exists (writeItem l v::x1). auto. }
+  }
+Qed. 
+
+Theorem validateHeapExtensionA : forall S L H S' new L' C e, 
+                  Forall (fun x : location * term * stamp => getStamp x = C) new ->
+                  S < C ->
+                  validate S L H S' H L' (abort e) ->
+                  validate S L (new++H) S' (new++H) L' (abort e) \/
+                  (exists Lnew e', validate S L (new++H) S' (new++H) Lnew (abort e') /\
+                             postfix Lnew L').
+Proof.
+  intros. remember (abort e). induction H2; try solve[inv Heqv]. 
+  {apply IHvalidate in H1; auto. inv H1. 
+   {left. eapply validateAbortPropogate. auto. }
+   {invertHyp. right. exists x0. exists x1. split; auto. eapply validateAbortPropogate. auto. }
+  }
+  {eapply validateHeapExtensionC in H3. inv H3. 
+   {invertHyp. left. eapply LookupExtensionGE in H4. Focus 2. eauto. inv H4. 
+    {eapply validateAbortRead; eauto. }
+    {invertHyp. eapply validateAbortRead; eauto. omega. }
+   }
+   {invertHyp. right. exists x. exists x0. split. eapply validateAbortPropogate; auto. auto. }
+   eauto. auto. 
+  }
+Qed. 
+
+Theorem trans_multistepLogMonotonic : forall H act L L' e e' S,
+                                        trans_multistep H (S, L,e) (S,L',e') ->
+                                        In act L -> In act L'. 
+Proof.
+  intros. dependent induction H0; auto. inv H0. 
+  {eapply IHtrans_multistep; auto. simpl. right. auto. }
+  {eapply IHtrans_multistep; auto. }
+  {eapply IHtrans_multistep; auto. simpl. right. auto. }
+  {eapply IHtrans_multistep; auto. }
+  {eapply IHtrans_multistep; auto. }
+Qed. 
+Theorem lookupSame : forall H' H l S S' C v v', 
+              Forall (fun x0 : location * term * stamp => getStamp x0 = C) H' ->
+              lookup H l = Some(v, S) -> S' < C -> S < C ->
+              lookup (H'++H) l = Some(v',S') -> v' = v /\ S' = S. 
+Proof.
+  induction H'; intros. 
+  {simpl in H4. eapply lookupDeterministic in H1; eauto. }
+  {simpl in *. destruct a. destruct p. destruct (eq_nat_dec l l0). 
+   {inv H4. inv H0. simpl in *. omega. }
+   {inv H0. simpl in H8. eauto. }
+  }
+Qed. 
+
+Theorem lookupValid : forall L H H' H'' l v S E S' S'0 C,
+              lookup H l = Some(v, S'0) ->
+              validate S L (H'++H) S' H'' L commit -> S < C -> S'0 < C ->
+              Forall (fun x0 : location * term * stamp => getStamp x0 = C) H' ->
+              In (readItem l E) L ->
+              lookup (H'++H) l = Some(v,S'0).
+Proof.
+  induction L; intros. 
+  {inv H5. }
+  {inv H5. 
+   {inv H1. eapply lookupSame in H0. Focus 2. eauto. Focus 3. auto. Focus 3. 
+    eauto. invertHyp. auto. omega. }
+   {inv H1; eapply IHL; eauto. }
+  }
+Qed. 
+
+Theorem trans_multiHeapExt : forall H H' S e0 e L S' L' e' C, 
+                 trans_multistep H (Some(S,e0),L,e) (Some(S,e0),L',e') ->
+                 (exists x, validate S L' (H'++H) S' x L' commit) ->
+                 Forall (fun x0 : location * term * stamp => getStamp x0 = C) H' ->
+                 S < C ->
+                 trans_multistep (H'++H) (Some(S,e0),L,e) (Some(S,e0),L',e').
+Proof.
+  intros. dependent induction H0.  
+  {constructor. }
+  {inv H0. 
+   {copy H1. eapply trans_multistepLogMonotonic in H0. Focus 2. simpl. left. auto.
+    invertHyp. eapply lookupValid in H12; eauto. econstructor.
+    eapply t_readStep; eauto. eauto. omega. }
+   {econstructor. eapply t_readInDomainStep; eauto. eauto. }
+   {econstructor. eapply t_writeStep; eauto. eapply IHtrans_multistep; eauto. }
+   {econstructor. eapply t_atomicIdemStep; eauto. eauto. }
+   {econstructor. eapply t_betaStep; eauto. eauto. }
+  }
+Qed. 
+
+Theorem validateValidate : forall S L H S' H' L' e, 
+                             validate S L H S' H' L' (abort e) ->
+                             exists H'', validate S L' H S' H'' L' (commit). 
+Proof.
+  intros. remember (abort e). induction H0; try solve[inv Heqv]. 
+  {inv Heqv. assert(abort e = abort e) by auto. apply IHvalidate in H1. invertHyp. 
+   exists x0. auto. }
+  {exists H'. assumption. }
+Qed. 
+
+Theorem thread_wf_Extension : forall H H' t C, 
+                 threadWF H t -> optLT (getThreadStamp t) C ->
+                 Forall (fun x0 : location * term * stamp => getStamp x0 = C) H' ->
+                 threadWF (H'++H) t. 
+Proof. 
+  intros. inv H0.  
+  {constructor. } 
+  {simpl in H1. eapply validateHeapExtensionC in H3; eauto. inv H3. 
+   {invertHyp. econstructor. eauto. eapply trans_multiHeapExt; eauto. }
+   {invertHyp. copy H3. eapply validateValidate in H0. 
+    copy H3. apply abortLogPostfix in H6. invertHyp. 
+    assert(trans_multistep H (Some (S, e0), [], e0) (Some (S, e0), x, x0)).
+    admit. eapply threadWFInvalid. eauto. eapply trans_multiHeapExt; eauto. }
+  }
+  {simpl in H1. copy H3. eapply validateHeapExtensionA in H3; eauto. inv H3. 
+   {eapply threadWFInvalid. eauto. copy H5. eapply validateValidate in H3. invertHyp. 
+    eapply trans_multiHeapExt; eauto. }
+   {invertHyp. eapply threadWFInvalid. eauto. copy H0. apply abortLogPostfix in H5. 
+    invertHyp. copy H0. apply validateValidate in H5. invertHyp.
+    admit. }
+  }
+Qed. 
+
+Theorem trans_stepWF : forall H t t', 
+                  threadWF H t -> trans_step H t t' -> threadWF H t'.
+Proof.
+  intros. inv H1. 
+  {inv H0. 
+   {econstructor. eapply validateCommitRead; eauto.  eapply trans_multistep_trans. 
+    eassumption. econstructor. eapply t_readStep; eauto. constructor. }
+   {eapply threadWFInvalid. eapply validateAbortPropogate; eauto. auto. }
+  }
+  {inv H0. econstructor; eauto. eapply trans_multistep_trans. eassumption. 
+   econstructor. eapply t_readInDomainStep; eauto. constructor. 
+   eapply threadWFInvalid. eauto.  eapply trans_multistep_trans. eassumption. 
+   econstructor. }
+  {inv H0. exfalso. apply H3. auto. 
+   {econstructor. econstructor. eauto. eapply trans_multistep_trans. eauto. 
+    econstructor. eapply t_writeStep; eauto. constructor. }
+   {eapply threadWFInvalid. eapply validateAbortPropogate. eauto. auto. }
+  }
+  {inv H0. exfalso. apply H3. auto. 
+   {econstructor. eauto. eapply trans_multistep_trans. eauto. econstructor. 
+    eapply t_atomicIdemStep; eauto. constructor. }
+   {eapply threadWFInvalid; eauto. }
+  }
+  {inv H0. exfalso. apply H3. auto. 
+   {econstructor. eauto. eapply trans_multistep_trans. eauto. econstructor. 
+    eapply t_betaStep; eauto. constructor. }
+   {eapply threadWFInvalid; eauto. }
+  }
+Qed. 
+
+Theorem trans_stepStampSame : forall H t t', trans_step H t t' -> 
+                                      getThreadStamp t = getThreadStamp t'. 
+Proof.
+  intros. inv H0; auto. Qed. 
+
+Theorem f_stepWF : forall C H T C' H' T', 
+                   poolWF C H T ->
+                   f_step C H T C' H' T' -> 
+                   poolWF C' H' T'. 
+Proof.
+  intros. induction H1.
+  {inv H0. InTac. invertHyp. constructor. auto. intros. inv H5. 
+   split. Focus 2. eapply trans_stepWF; eauto.
+   erewrite <- trans_stepStampSame; eauto. }
+  {copy H0. apply wfPar_l in H0. apply IHf_step in H0. 
+   apply wfPar_r in H2. apply wfParConj. assumption. constructor. inv H0.
+   assumption. intros. inv H2. apply H6 in H3. copy H1. 
+   eapply stampHeapMonotonic in H1. invertHyp. split. Focus 2. 
+   eapply thread_wf_Extension; eauto. destruct (getThreadStamp t); auto. 
+   simpl in *. omega. }
+  {copy H0. apply wfPar_r in H0. apply IHf_step in H0. 
+   apply wfPar_l in H2. apply wfParConj; auto. constructor. inv H0.
+   assumption. intros. inv H2. apply H6 in H3. copy H1. 
+   eapply stampHeapMonotonic in H1. invertHyp. split. Focus 2.
+   eapply thread_wf_Extension; eauto. destruct (getThreadStamp t); auto. simpl in *. 
+   omega. }
+  {constructor. inv H0. auto. intros. inv H2. inv H6. split; simpl; auto.
+   constructor. inv H6. split; simpl; auto. constructor. }
+  {constructor. inv H0. eapply monotonicWeakening. Focus 2. eauto. omega. 
+   intros. inv H0. inv H2. copy H1. eapply abortLogPostfix in H1.
+   econstructor. simpl. auto. econstructor. constructor. constructor. }
+  {constructor. inv H0. constructor. omega. auto. intros. inv H0. inv H3. split. 
+   simpl. auto. constructor. }
+  {inv H0. constructor. eapply validateMonotonic; eauto. intros. inv H0. 
+   split. simpl. auto. constructor. }
+  {econstructor. inv H0. eapply monotonicWeakening;[idtac|eauto]. omega. intros. 
+   inv H2. split. simpl. auto. econstructor. constructor. econstructor. }
+  {constructor. inv H0. auto. intros. inv H2. split. simpl. auto. constructor. }
+  Grab Existential Variables. constructor. constructor. 
+Qed. 
+
+Theorem f_multistepWF : forall C H T C' H' T', 
+                   poolWF C H T ->
+                   f_multistep C H T C' H' T' -> 
+                   poolWF C' H' T'. 
+Proof.
+  intros. induction H1. auto. eapply f_stepWF in H1; auto. 
+Qed. 
+
+
+
+
+
+
+
+
+
+
+
+
+
+
+
+
+
+
+
+
+
+
+
+
